\documentclass[letterpaper]{article}
\usepackage[top=.5in, bottom=.5in, left=.5in, right=.5in]{geometry}
\usepackage[fleqn]{amsmath}
\usepackage{amsfonts,amssymb,amsthm}
\usepackage{multicol}
\usepackage{amsthm}
\usepackage{algorithmic}
\usepackage{ulem}
\usepackage{cancel}

\setlength{\parindent}{0in}
\setlength{\parskip}{0ex}
% \setlength{\abovedisplayskip}{-2ex}
% \setlength{\belowdisplayskip}{-2ex}
\setlength{\jot}{.5ex} 
% \linespread{0.5}

\providecommand{\abs}[1]{\left\lvert#1\right\rvert}
\providecommand{\norm}[1]{\left\lVert#1\right\rVert}
\providecommand{\inner}[1]{\left(#1\right)}
\providecommand{\ainner}[2]{\left\langle#1\,,#2\right\rangle}

\def\d{\mathrm{d}}
\def\U{\mathcal{U}}

\pagestyle{empty}
\begin{document}
\begin{multicols}{2}
\scriptsize
\setlength\abovedisplayskip{1pt plus 1pt minus 1pt}
\setlength\belowdisplayskip{1pt plus 1pt minus 1pt}
%%%%%%%%%%%%%%%%% ODEs %%%%%%%%%%%%%%%%%%%%%%%%%%%%%%%%%%%%%
Euler
\[
\norm{e_{n+1}}\le(1+h\lambda)\norm{e_n}+Ch^2
\]
\begin{align*}
\norm{e_n}&\le\frac{C}{\lambda}h\left[(1+h\lambda)^n-1\right]\\
&\le\frac{C}{\lambda}(e^{T\lambda}-1)h
\end{align*}
Trapezoid
\[
\norm{e_{n+1}}\le\left(\frac{1+\frac{1}{2}h\lambda}{1-\frac{1}{2}h\lambda}\right)\norm{e_n}+\left(\frac{C}{1-\frac{1}{2}h\lambda}\right)h^3
\]
\[
\norm{e_n}\leq\frac{C}{\lambda}\left[\left(\frac{1+\frac{1}{2}h\lambda}{1-\frac{1}{2}h\lambda}\right)^n-1\right]h^2
\]
General s-step
\[
\sum_{m=0}^sa_my_{n+m}=h\sum_{m=0}^sb_mf(t_{n+m},y_{n+m})
\]
\begin{align*}
\rho(w)&=\sum_{m=0}^sa_mw^m\\
\sigma(w)&=\sum_{m=0}^sb_mw^m
\end{align*}
Order p iff
\[
\rho(\xi+1)-\sigma(\xi+1)\ln(\xi+1)=c(\xi)^{p+1}+\mathcal{O}(\xi^{p+2})
\]
Root Condition: all zeros reside in closed complex unit disc and all zeros of
unit modulus are simple.
\[
\norm{f(x)-p(x)}_{L^\infty}\le\frac{(b-a)^s}{s!}\norm{f^{(s)}}_{L^\infty}
\]

Runge-Kutta
\[
\xi_j=y_n+h\sum_{i=1}^\nu a_{j,i}f(t_n+c_ih,\xi_i)
\]
\[
y_{n+1}=y_n+h\sum_{j=1}^\nu b_jf(t_n+c_jh,\xi_j)
\]
\[
\begin{array}{c|c}
\mathbf{c} & A\\
\hline
& \mathbf{b}^T
\end{array}
\]

Collocation
\[
\int_0^1\tau^j\prod_{l=1}^\nu(\tau-c_l)=0\,,\quad j=0,1,\dots,m-1
\]
for some $m\in\{0,1,\dots,\nu\}$. Then the collocation method is of order
$\nu+m$.
\[
q(t)=\prod_{j=1}^\nu(t-c_j)\,,\quad q_l(t)=\frac{q(t)}{t-c_l}
\]
\[
a_{j,i}=\int_0^{c_j}\frac{q_i(\tau)}{q_i(c_i)}\d\tau\,,\quad    
b_j=\int_0^1\frac{q_j(\tau)}{q_j(c_j)}\d\tau
\]
Let $c_1,c_2,\dots,c_\nu$ be the zeros of the polynomials that are orthogonal
with respect to the weight function $\omega(t)\equiv 1\,,0\le t\le1$. Then the
underlying collocation method is of order $2\nu$.

Stability of Runge-Kutta Methods
\[
r(z)=1+z\mathbf{b}^T(I-zA)^{-1}\mathbf{1}
\]
\[
(I-zA)^{-1}=\frac{\mathrm{adj}(I-zA)}{\det(I-zA)}
\]
Adjugate is transpose of cofactor matrix

$\abs{r(z)}<1$ for all $z\in\mathbb{C}^-$ iff all the poles of $r$ have positive
real parts and $\abs{r(it)}\le 1$ for all $t\in\mathbb{R}$.

Multistep methods
\[
\eta(z,w)=\sum_{m=0}^s(a_m-b_mz)w^m
\]
The multistep method is A-stable iff $b_s>0$ and
\[
\abs{w_1(it)},\,\abs{w_2(it)},\dots,\abs{w_{q(it)}(it)}\le 1\,,\quad
t\in\mathbb{R}
\]
where $w_1,\,w_2,\dots,w_{q(z)}$ are the zeros of $\eta(z,\cdot)$.

Linearizing a non-linear equation
\[
y'=\underbrace{f(t,y)}_{b}+\underbrace{\nabla f(t,y)}_{A}(y-\bar y)
+\mathcal{O}(\abs{y-\bar y}^2)
\]
Solution of nonlinear equations

Fixed Point
\[
\mathbf{w}=h\mathbf{g}(\mathbf{w})+\boldsymbol\beta
\]
Unique solution exists in sufficiently small neighborhood of $\beta$ if
$\left(\mathbf{I}-h\frac{\partial\mathbf{g}}{\partial\mathbf{w}}\right)$ is
nonsingular.

\textbf{Banach Fixed Point Theorem}
If $G:\mathbb{R}^d\rightarrow\mathbb{R}^d$ is a contraction: $\exists
0\le\lambda<1$ s.t.
\[
\norm{G(u)-G(v)}\le\lambda\norm{u-v}\quad\forall u,v\in\mathbb{R}^d
\]
Then $\exists!$ fixed point $w$ and 
\[
\norm{w^i-w}\le\lambda^i\norm{w^0-w}
\]

If $g$ is Lipshitz with constant $\Lambda$, we need
$h\le\frac{\lambda}{\Lambda}$

Newton's Method
\[
w^{i+1}=w^i-\frac{F(w^i)}{F'(w^i)}
\]
\[
w^{i+1}=w^i-\left(\frac{\partial F(w)}{\partial w}\right)^{-1}F(w^i)
\]

%%%%%%%%%%%%%%%%%%%%%%%%%% Elliptic Equations %%%%%%%%%%%%%%%%%%%%%%%%%%%%%%%%%%%%%
\uline{Continuous (bounded)}
\[
\exists\eta^*>0\text{ s.t. }\abs{a(u,v)}\le\eta^*\norm{u}_H\norm{v}_H\,,\forall
u,v\in H
\]

\uline{Coercive}
\[
\exists\eta_*>0\text{ s.t. }a(u,u)\ge\eta_*\norm{u}_H^2\,,\forall u\in H
\]

\uline{Energy Norm}
If $a(u,v)$ is bilinear, continuous, coercive, and symmetric it defines a norm
\[
\norm{u}_E=\sqrt{a(u,u)}
\]
\[
\sqrt{\eta_*}\norm{u}_H\le\norm{u}_E\le\sqrt{\eta^*}\norm{u}_H
\]

\uline{Lax-Milgram}
If H is Hilbert,
$a:H\times H\rightarrow\mathbb{R}$ is bilinear, bounded, coercive
and $F:H\rightarrow\mathbb{R}$ is linear, bounded, then $\exists! w\in H$ s.t.
\[
a(w,v)=F(v)\,,\quad\forall v\in H
\]

\uline{Poincar\`e Inequality} If $\Omega\subset\mathbb{R}^d$ bounded then
$\exists\quad C(\Omega)\,,C'(\Omega)>0$ s.t.
\begin{align*}
\norm{v}_{L_2}&\le C(\Omega)\norm{\nabla v}_{L_2}\,,\quad\forall v\in
H_0^1(\Omega)\\
\norm{v}_{H^1}&\le C'(\Omega)\norm{\nabla v}_{L_2}\,,\quad\forall v\in
H_0^1(\Omega)
\end{align*}

\uline{BVP Solvability} Given $\Omega\subset\mathbb{R}^d$ bounded with Lipshitz
boundary, $\Gamma_D=\Gamma$, $\tilde g_D\in H^1(\Omega)$ and $f\in
H^{-1}(\Omega)$. Consider the problem of finding $u=\tilde u+\tilde h_d$,
$\tilde u\in H_0^1(\Omega)$ s.t.
\[
\inner{\uuline{a}\nabla u}{\nabla v}+\inner{bu}{\nabla
v}+\inner{cu}{v}=\ainner{f}{v}\,,\quad \forall v\in H_0^1(\Omega)
\]
or 
\[
\underbrace{\inner{\uuline{a}\nabla\tilde u}{\nabla v}+\inner{b\tilde u}{\nabla
v}+\inner{c\tilde u}{v}}_{a(\tilde u,v)}
=\underbrace{\ainner{f}{v}-a(\tilde g_D,v)}_{F(v)}
\]
\begin{enumerate}
\item If $\uuline{a}\in L_\infty(\Omega)^{d\times d}$, $b\in L_\infty(\Omega)^d$
and $c\in L_\infty(\Omega)$ then $a(\tilde u, v)$ and $F(v)$ are bounded.
\item Additionally, if $\uuline{a}$ is symmetric and uniformly positive
definite, $c\ge0$ and $\norm{b}_\infty<\frac{a_*}{C(\Omega)}$ then $a(\tilde
u,v)$ is coercive.
\item Additionally, if $b\equiv 0$, then $a(\tilde u,v)$ is symmetric and there
is an energy $J(\cdot)$, inner product $a(\cdot,\cdot)$ and norm
$\norm{\cdot}_E$ associated with the problem
\end{enumerate}
By Lax-Milgram: 1. + 2. $\Rightarrow\exists!$ solution $u=\tilde u+\tilde g_D$

1. + 2. + 3. $\Rightarrow\quad\tilde u$ is a strict minimum of $J$

\uline{Proof of 1.}
\begin{align*}
\abs{a(\tilde u,v)}&\le\abs{(\uuline{a}\nabla\tilde u,\nabla v)}
+\abs{(b\tilde u,\nabla v)}+\abs{(c\tilde u,v)}\\
&\le\int_\Omega\abs{\uuline{a}\nabla\tilde u\cdot v}\d\Omega
+\int_\Omega\abs{b\tilde u\cdot \nabla v}\d\Omega
+\int_\Omega\abs{c\tilde u v}\d\Omega\\
&\le\int_\Omega\abs{\uuline{a}\nabla\tilde u}\abs{\nabla v}\d\Omega
+\int_\Omega\abs{b\tilde u}\abs{\nabla v}\d\Omega
+\int_\Omega\abs{c\tilde u}\abs{v}\d\Omega\\
&\le||\uuline{a}||_\infty\inner{\abs{\nabla\tilde u}}{\abs{\nabla v}}
+||b||_\infty\inner{\abs{\tilde u}}{\abs{\nabla v}}
+||c||_\infty\inner{\abs{\tilde u}}{\abs{v}}\\
&\le||\uuline{a}||_\infty\norm{\nabla \tilde u}_{L_2}\norm{\nabla v}_{L_2}
+||b||_\infty\norm{\tilde u}\norm{\nabla v}
+||c||_\infty\norm{\tilde u}\norm{v}\\
&\le\underbrace{(||\uuline{a}||_\infty+||b||_\infty+||c||_\infty)}_{\eta^*>0}
\norm{\tilde u}_{H^1}\norm{v}_{H^1}\\
\end{align*}
\begin{align*}
\abs{F(v)}&\le\abs{\langle f,v\rangle}+\abs{a(\tilde g,v)}\\
&\le C\norm{v}_{H^1}+\eta^*\norm{\tilde g_D}_{H^1}\norm{v}_{H^1}\,,\quad\quad f\in H^{-1}\\
&\le \hat C\norm{v}_{H^1}
\end{align*}

\uline{Proof of 2.}
\begin{align*}
a(v,v)&\ge(\uuline{a}\nabla v,\nabla v)+(bv,\nabla v)+(cv,v)\\
&\ge\uuline{a}_*\norm{\nabla v}_{L_2}^2-\abs{(bv,\nabla v)}+(cv,v)\,,
\text{ Cauchy-Schwarz}\\
&\ge\uuline{a}_*\norm{\nabla v}_{L_2}^2
-\norm{b}_\infty\norm{v}_{L_2}\norm{\nabla v}_{L_2}\,,\text{ Poincare}\\
&\ge\uuline{a}_*\norm{\nabla v}_{L_2}^2
-\norm{b}_\infty C(\Omega)\norm{\nabla v}_{L_2}\\
&\ge\left(\frac{\uuline{a}_*}{C(\Omega}
-\norm{b}_\infty\right) C(\Omega)\norm{\nabla v}_{L_2}\\
&\ge\left(\frac{\uuline{a}_*}{C(\Omega}
-\norm{b}_\infty\right)\frac{C(\Omega)}{(C'(\Omega))^2}\norm{v}_{H^1}\\
&\ge\eta_*\norm{v}_{H^1}^2\,,\quad\forall v\in H_0^1(\Omega)
\end{align*}

\uline{Stability} Choose $v=u_h-g\in V_h$
\begin{align*}
a(u_h,u_h-g)&=f(u_h-g)\\
a(u_h-g,u_h-g)&=f(u_h-g)-a(g,u_h-g)\\
a_*\norm{u_h-g}_V^2&\le\norm{f}_V\norm{u_h-g}_V+a^*\norm{g}_V\norm{u_h-g}_V\\
\norm{u_h-g}_V&\le\frac{\norm{f}_V+a^*\norm{g}_V}{a_*}
\end{align*}

\uline{Error Estimation} 
\[
a(u-u_h,v)=0\,,\quad\forall v\in V_h
\]
Take $v\mapsto u-u_h-(u-v)\,,\quad v\in V_h$
\begin{align*}
a(u-u_h,u-u_h)&=a(u-u_h,u-v)\,,\quad\forall v\in V_h\\
a_*\norm{u-u_h}_V^2&\le a^*\norm{u-u_h}_V\norm{u-v}_V\,,\quad\forall v\in V_h\\
\norm{u-u_h}_V&\le\frac{a^*}{a_*}\norm{u-v}_V\,,\quad\forall v\in V_h\\
\end{align*}

\uline{Cea's Lemma} 
\[
\norm{u-u_h}_V\le\left(\frac{a^*}{a_*}\right)\inf_{v\in V_h}\norm{u-v}_V
\]
\uline{Galerkin Orthogonality}
\[
a(u-u_h,v)=0\,,\quad\forall v\in V_h
\]
\uline{Theorem}
\[
\norm{u-u_h}_a=\inf_{v\in V_h}\norm{u-v}_a
\]
\uline{Proof}
\begin{align*}
\norm{u-u_h}_a^2&=a(u-u_h,u-uh)\\
&=a(u-u_h,u-v)+\cancel{a(u-u_h,v-u_h)}\\
&\le\norm{u-u_h}_a\norm{u-v}_a
\end{align*}

\uline{Ciarlet FEM Definition} Let
\begin{enumerate}
\item $E\subseteq\mathbb{R}^d$ domain with piecewise smooth boundary
\item $\mathcal{P}$ is a finite dimensional vector space of functions on $E$
(shape functions)
\item $\mathcal{N}=\{N_1,\dots,N_k\}$ is a basis for $\mathcal{P}'$, a set of
linear functionals on $\mathcal{P}$ (nodal variables or DOFs)
\end{enumerate}
Then $(E,\mathcal{P},\mathcal{N})$ is a finite element

\uline{Definition} Let $\{\phi_1,\dots,\phi_k\}$ be a basis for $\mathcal{P}$
dual to $\mathcal{N}$, $(N_i(\phi_j)=\delta_{ij})$

\uline{Unisolvence} If $\mathrm{dim}\mathcal{P}=k$ and
$\{N_1,\dots,N_k\}\subseteq\mathcal{P}'$

$\{N_1,\dots,N_k\}$ is a basis iff

$N_i(v)=0\,,\quad\forall i\,,\text{ then }v=0$

\uline{Peano Kernel Theorem}
If $L$ is a continuous linear functional on $C^{k+1}(a,b)$ s.t.
$L(p)=0\,,\forall p\in\mathbb{P}$. Then
\[
L(f)=\int_a^b f^{(k+1)}(\xi)K(\xi)\d\xi
\]
\[
K(\xi)=\frac{1}{k!}L\left( (\cdot-\xi)^k_+ \right)
\]

%%%%%%%%%%%%%%%%%%%%%%%% Parabolic Equations %%%%%%%%%%%%%%%%%%%%%%%%%%%%%%%%%%%%%
Stability:
\begin{align*}
\inner{\frac{u^n-u^{n-1}}{\Delta t}\,,u^n}+\inner{a\nabla u^n\,,\nabla u^n}
=\inner{f\,,u^n}
\end{align*}
\begin{align*}
\inner{u^n,u^n}-\inner{u^{n-1},u^{n-1}}&\le2\Delta t\norm{f^n}_0\norm{u^n}_0\\
&\le\frac{\Delta t}{\epsilon}\norm{f^n}_0^2+\epsilon\norm{u^n}_0^2\Delta t\\
\end{align*}
\begin{align*}
\norm{u^M}_0^2-\norm{u^0}_0^2
&\le\sum_{n=1}^M\frac{\Delta t}{\epsilon}\norm{f^n}_0^2
+\sum_{n=1}^M\epsilon\norm{u^n}_0^2\Delta t\\
&\le\sum_{n=1}^M\frac{\Delta t}{\epsilon}\norm{f^n}_0^2
+M\Delta t\epsilon\max_n\norm{u^n}_0^2\\
\max_n\norm{u^n}_0^2&\le \frac{T}{\epsilon}\max_n\norm{f^n}_0^2+\norm{u^0}_0^2
\end{align*}
Convergence: 
Find $u^n\in V+g^n$ s.t.
\begin{align*}
\inner{c\frac{u^n-u^{n-1}}{\Delta t}\,,v}+\inner{a\nabla u^n\,,\nabla v}
=\inner{f^n\,,v}\\
+\inner{c\inner{\frac{u^n-u^{n-1}}{\Delta t}-u_t^n}\,, v}\,, \quad\forall v\in V
\end{align*}
Find $u_h^n\in V_h+g^n$ s.t.
\begin{align*}
\inner{c\frac{u_h^n-u_h^{n-1}}{\Delta t}\,,v}+\inner{a\nabla u_h^n\,,\nabla v}
=\inner{f^n\,,v} \,, \quad\forall v\in V_h
\end{align*}
\[
\inner{c\frac{\zeta^n-\zeta^{n-1}}{\Delta t}\,,v}
+\inner{a\nabla\zeta^n\,,\nabla v}
=\inner{c\inner{\frac{u^n-u^{n-1}}{\Delta t}-u_t^n}\,,v}
\]
$\inner{a\nabla(\tilde u-u)\,,\nabla v}=0\,,\quad\forall v\in V_h$
\begin{align*}
&\inner{c\tilde\zeta^n\,,\tilde\zeta^n}-\inner{c\tilde\zeta^{n-1}\,,\tilde\zeta^{n-1}}
+2\Delta t\inner{a\nabla\tilde\zeta^n\,,\nabla\tilde\zeta^n}\\
&\le 2\Delta t\inner{c\inner{\frac{u^n-u^{n-1}}{\Delta t}-u_t^n}\,,\tilde\zeta^n}
+2\Delta t\inner{c\inner{\tilde u_t^n-u_t^n}\,,\tilde\zeta^n}\\
&\le c^*\Delta t
\norm{\frac{\tilde u^n-\tilde u^{n-1}}{\Delta t}-\tilde u_t^n}_0^2
+c^*\Delta t\norm{\tilde u_t^n-u_t^n}_0^2
+2\frac{c^*}{c_*}\Delta t\inner{c\tilde\zeta^n\,,\tilde\zeta^n}\\
&\le\underbrace{\sum_{k=1}^nc^*\Delta t\left\{
\norm{\frac{\tilde u^k-\tilde u^{k-1}}{\Delta t}-\tilde u_t^k}_0^2
+\norm{\tilde u_t^k-u_t^k}_0^2\right\}}_{a^n}\\
&+\underbrace{\sum_{k=1}^{n-1}c^*\Delta t\left\{
\norm{\frac{\tilde u^k-\tilde u^{k-1}}{\Delta t}-\tilde u_t^k}_0^2
+\norm{\tilde u_t^k-u_t^k}_0^2\right\}}_{a^{n-1}}
+\underbrace{2\frac{c^*}{c_*}}_{b^n}
\Delta t\underbrace{\inner{c\tilde\zeta^n\,,\tilde\zeta^n}}_{u^n}
\end{align*}

\begin{align*}
\norm{\frac{\tilde u^n-\tilde u^{n-1}}{\Delta t}-\tilde u_t^n}^2&=
\frac{1}{\Delta t}\norm{\int_{t_{n-1}}^{t_n}(\tilde u_t(\tau)-\tilde
u_t^n)\d\tau}^2\\
&=\frac{1}{\Delta t}\norm{\int_{t_{n-1}}^{t_n}-\int_\tau^{t_n}\tilde u_{tt}(s)\d
s\d\tau}^2\\
&\le\int_{t_{n-1}}^{t_n}\norm{\tilde u_{tt}(\tau)}^2\d\tau(\Delta t)^2
\end{align*}

\begin{align*}
u^N&\le a^N\inner{1+\sum_{n=1}^Nb^nC_1\Delta t}\le C_2 a^N\\
&\le C_2\left(c^*\norm{\tilde u_{tt}}^2_{L^2(L^2)}\Delta t^2+C_3h^4\right)\\
&\le C\cdot\mathcal{O}(\Delta t^2+h^4)
\end{align*}

Gronwall: If
\[
u'(t)\le a(t)+b(t)u(t)\,,\quad\forall t\ge0
\]
where $b(t)\ge0$, then
\[
u(t)\le e^{\int_0^tb(\tau)\d\tau}\left\{u(0)+
\int_0^ta(\tau)e^{\int_0^\tau b(s)\d s}\d\tau\right\}
\]
% \uline{Corollary} If
% \[
% u(t)\le a(t)+\int_0^tb(\tau)u(\tau)\d\tau
% \]
% where $a\,,b\ge0$, then
% \[
% u(t)\le a(t)+\int_0^t a(\tau)b(\tau)e^{t-\tau}\d\tau
% \]
Discrete Gronwall: If
\[
\frac{u^n-u^{n-1}}{\Delta t}\le\frac{a^n-a^{n-1}}{\Delta
t}+b^nu^n\,,\quad\forall n\ge 1\,,\quad u^0=a^0=0
\]
where $a^n\,,b^n\ge0\,,\quad\forall n$, then, for $\Delta t\ge0$ sufficiently
small,
\[
u^N\le a^N+\sum_{n=1}^Na^nb^n\frac{\prod_{j=1}^{n-1}(1-b^j\Delta
t)}{\prod_{j=1}^N(1-b^j\Delta t)}\Delta t
\]

%%%%%%%%%%%%%%%%%%%%%%% Hyperbolic Equations %%%%%%%%%%%%%%%%%%%%%%%%%%%%%
Fourier Transform
\[
\hat w(\theta)=\sum_{j=-\infty}^\infty w_je^{-ij\theta}
\]
\[
w_j=\frac{1}{2\pi}\int_0^{2\pi}\hat w(\theta)e^{ij\theta}\d\theta
\]
Particle Velocity: $f(u)/u$\\
Characteristic Velocity: $f'(u)$\\
Characteristics: $x(t)$ where $u$ is constant $x'(t)=f'(u(x(t),t))$\\
$x_\xi(t)=u_0(\xi)t+\xi$\\
Find CFL such that Lax-Wendroff is stable
\begin{align*}
\U_j^{n+1}=\U_j^n-\frac{a\Delta t}{2h}\left(\U_{j+1}^n-\U_{j-1}^n\right)
+\frac{a^2(\Delta t)^2}{2h^2}\left(\U_{j+1}^n-2\U_j^n+\U_{j-1}^n\right)
\end{align*}
\begin{align*}
\hat\U^{n+1}=\hat\U^n\left[1-\lambda i\sin\theta+\lambda^2(\cos\theta-1)\right]
\end{align*}
\begin{align*}
\abs{1-\lambda i\sin\theta+\lambda^2(\cos\theta-1)}^2
&=(1+\lambda^2(\cos\theta-1))^2+\lambda^2\sin^2\theta\le1
\end{align*}
% Box Method: $(1-\lambda)\U_{j-1}^{n+1}+(1+\lambda)\U_j^{n+1}=(1+\lambda)\U_{j-1}^n+(1-\lambda)\U_j^n$
Rankine-Hugoniot Jump Condition $M>>st$
\[
\frac{\d}{\d t}\int_{-M}^Mu(x,t)\d x=(M+st)u_L+(M-st)u_R=f(u_L)-f(u_R)
\]
\[
s=\frac{f(u_L)-f(u_R)}{u_L-u_R}
\]
Rarefaction
\[
\frac{f(u)-f(u_L)}{u-u_L}\ge s\ge\frac{f(u)-f(u_R)}{u-u_R}
\]
Average flux entering $(x_{i+1/2},x_{i+3/2})$: $\frac{1}{\Delta
t}\int_{t_n}^{t_{n+1}}f(u_{i+1/2})\d x$\\
Conservative Method
\[
\frac{\U_i^{n+1}-\U_i^n}{\Delta
t}+\frac{1}{h}\left\{F(\U_{i-p}^n,\U_{i-p+1}^n,\dots,\U_{i+q})
-F(\U_{i-p-1}^n,\U_{i-p}^n,\dots,\U_{i+q-1})\right\}=0
\]
\end{multicols}
\end{document}

